\item $x\left(p\right) \geqslant 0 \ \wedge \  y\left(p\right) \geqslant 0 \ \Leftrightarrow \ \theta \in \left\langle 0;\frac{\pi}{2}\right\rangle$
  		\begin{align*}
        	\alpha\left( p\right) & = \frac{
        		y\left(p\right)
        	}{
        		d\left(p\right)
        	} = \frac{
        		y\left(p\right)
        	}{
        		\left|x\left(p\right)\right| + \left|y\left(p\right)\right|
        	} = \frac{
        		y\left(p\right)
        	}{
        		x\left(p\right) + y\left(p\right)
        	} & \hspace{10cm}\\
        	\gamma\left( \theta\right) & = \alpha\left( p\left(\theta\right) \right) = \frac{
        		\left|R\right| \cdot \sin \theta
        	}{
        		\left|R\right| \cdot \cos \theta + \left|R\right| \cdot \sin \theta
        	} =\frac{
        		\sin \theta
        	}{
        		\sin \theta + \cos \theta
        	} \\
        	\frac{
        		d
        	}{
        		d\theta
        	}\gamma\left( \theta\right) & = \frac{
        		d
        	}{
        		d\theta
        	}\left(
        		\frac{ 
        			\sin \theta
        		}{
        			\sin \theta + \cos \theta
        		}
        	\right) \\ 
        	& =\frac{
        		\frac{
        			d
        		}{
        			d\theta
        		}\left(
        			\sin\theta
        		\right)\cdot\left(
        			\sin \theta + \cos \theta
        		\right)
        		-\sin\theta\cdot\frac{
        			d
        		}{
        			d\theta
        		}\left(\sin \theta + \cos \theta\right)
        	}{
        		\left(
        			\sin \theta + \cos \theta
        		\right)^2
        	}\\
        	& =\frac{
        		\cos\theta\cdot\left(\sin \theta + \cos \theta\right)
        		-\sin\theta\cdot\left(\cos \theta - \sin \theta\right)
        	}{
        		\sin^2 \theta + 2\sin\theta\cos\theta + \cos^2 \theta 
        	}\\
        	& =\frac{
        		\cos\theta\sin \theta + \cos^2 \theta
        		-\sin\theta\cos \theta  + \sin^2 \theta
        	}{
        		1 + 2\sin\theta\cos\theta
        	} = \frac{
        		1
        	}{
        		1 + 2\sin\theta\cos\theta
        	} \\
        	& = \frac{
        		1
        	}{
        		1 + \sin 2\theta
        	} 
        \end{align*}
        \begin{align*}
        	\frac{d}{d\theta}\gamma\left( \theta\right)& > 0& \hspace{10cm}\\
        	\frac{
        		1
        	}{
        		1 + \sin 2\theta
        	} & > 0\\
        	1 + \sin 2\theta & > 0\\
        	 \sin 2\theta & > -1\\
        	 \sin 2\theta & \neq -1\\
        	 2\theta & \neq \frac{3}{2}\pi + 2k\pi\\
        	 \theta & \neq \frac{3}{4}\pi + k\pi ; \ k \in \mathbb{Z}
        \end{align*}
       	\begin{align*}
       		\left. \begin{array}{rcl}
       		 k = 0 & \Rightarrow & \theta \neq \frac{3}{4}\pi > \frac{\pi}{2}  \\
    	 	 k = -1 & \Rightarrow &\theta \neq -\frac{1}{4}\pi < 0
    	 	\end{array}    \right\}\Rightarrow \frac{d}{d\theta}\gamma\left( \theta\right) > 0 \text{ dla } \theta \in \left\langle 0;\frac{\pi}{2}\right\rangle& \hspace{10cm}
        \end{align*}
       	\begin{align*}
       	\left. \begin{array}{rcl}
       		\gamma\left( 0\right) & = &\frac{\sin 0}{\sin 0 + \cos 0} = \frac{0}{0 + 1} = 0\\	
       		\gamma\left( \frac{\pi}{2}\right) & = &\frac{\sin  \frac{\pi}{2}}{\sin  \frac{\pi}{2} + \cos  \frac{\pi}{2}} = \frac{1}{1 + 0}= 1
       	\end{array} \right\} \Rightarrow \gamma\left( \theta\right) \in \left\langle 0;1\right\rangle \text{ dla } \theta \in \left\langle 0;\frac{\pi}{2}\right\rangle& \hspace{10cm}
        \end{align*}