\item $x\left(p\right) < 0 \ \wedge \ y\left(p\right) < 0 \ \Leftrightarrow \ 
  		\theta \in \left( \pi;\frac{3\pi}{2}\right)$\\
  		\alignspace
  		\begin{align*} 
        	\alpha\left( p\right) 
        	& = 2 + \frac{
        		\left|
        			y\left(p\right)
        		\right|
        	}{
        		d\left(p\right)
        	} = 2 + \frac{
        		- y\left(p\right)
        	}{
        		\left|x\left(p\right)\right| + \left|y\left(p\right)\right|
        	} = 2 - \frac{
        		y\left(p\right)
        	}{
        		-x\left(p\right) - y\left(p\right)
        	} & \hspace{10cm}\\
        	& = 2 + \frac{
        		y\left(p\right)
        	}{
        		x\left(p\right) + y\left(p\right)
        	}\\
        	\gamma\left( \theta\right) & = \alpha\left( p\left(\theta\right) \right) = 2 + \frac{
        		\left|R\right| \cdot \sin \theta
        	}{
        		 \left|R\right| \cdot \cos \theta 
        		 + \left|R\right| \cdot \sin \theta
        	} = 2 + \frac{
        		\sin \theta	
        	}{
        		 \sin \theta + \cos \theta
        	} \\
        	\frac{
        		d
        	}{
        		d\theta
        	}\gamma\left( \theta\right) & = \frac{
        		d
        	}{
        		d\theta
        	}\left( 2 + \frac{
        			\sin \theta	
        		}{
        		 	\sin \theta + \cos \theta
        		}
        	\right) \\ 
        	& =\frac{
        		\frac{
        			d
        		}{
        			d\theta
        		}\left(
        			\sin\theta
        		\right)\cdot\left(
        			\sin \theta + \cos \theta
        		\right)
        		-\sin\theta\cdot\frac{
        			d
        		}{
        			d\theta
        		}\left(\sin \theta + \cos \theta\right)
        		}{
        		\left(
        			\sin \theta + \cos \theta
        		\right)^2
        		}\\
        	& =\frac{
        		\cos\theta\cdot\left(\sin \theta + \cos \theta\right)
        		-\sin\theta\cdot\left(\cos \theta - \sin \theta\right)
        	}{
        		\sin^2 \theta + 2\sin\theta\cos\theta + \cos^2 \theta 
        	}\\
        	& =\frac{
        		\cos\theta\sin \theta + \cos^2 \theta
        		-\sin\theta\cos \theta  + \sin^2 \theta
        	}{
        		1 + 2\sin\theta\cos\theta
        	}\\
        	& = \frac{
        		 \cos^2 \theta
        		+ \sin^2 \theta
        	}{
        		1 + 2\sin\theta\cos\theta
        	} =\frac{
        		1
        	}{
        		1 + \sin 2\theta
        	}
        \end{align*}\alignspace
        \begin{align*}
        	\frac{d}{d\theta}\gamma\left( \theta\right)& > 0& \hspace{10cm}\\
        	\frac{
        		1
        	}{
        		1 + \sin 2\theta
        	} & > 0\\
        	1 + \sin 2\theta & > 0\\
        	 \sin 2\theta & > -1\\
        	 \sin 2\theta & \neq -1\\
        	 2\theta & \neq \frac{3}{2}\pi + 2k\pi\\
        	 \theta & \neq \frac{3}{4}\pi + k\pi ; \ k \in \mathbb{Z}
        \end{align*}\alignspace
       	\begin{align*}
       		\left. \begin{array}{rcl}
       		 k = 0 & \Rightarrow & \theta \neq \frac{3}{4}\pi < \pi  \\
    	 	 k = 1 & \Rightarrow &\theta \neq \frac{7}{4}\pi > \frac{3\pi}{2}
    	 	\end{array}    \right\}\Rightarrow \frac{d}{d\theta}\gamma\left( \theta\right) > 0 \text{ dla } \theta \in \left( \pi;\frac{3\pi}{2}\right)& \hspace{10cm}
        \end{align*}\alignspace
       	\begin{align*}
       	\left. \begin{array}{rcl}
       		\gamma\left( \pi\right) & = &
       		 2 + \frac{\sin \pi}{\sin \pi + \cos \pi } 
       		 =2 - \frac{0}{0 - 1} = 2\\	
       		\gamma\left( \frac{3\pi}{2}\right) & = &
       		2 + \frac{\sin  \frac{3\pi}{2}}{\sin  \frac{3\pi}{2} + \cos \frac{3\pi}{2}}\\
       		& = & 2 + \frac{-1}{-1 + 0}= 2 + 1 = 3
       	\end{array} \right\} \Rightarrow \gamma\left( \theta\right) \in \left( 2;3\right) \text{ dla } \theta \in \left( \pi;\frac{3\pi}{2}\right)& \hspace{10cm}
        \end{align*}